prove lemmas about the inode 'heap' in dir_proof

src/program_proof/examples/dir_proof.v
@@ -28,21 +28,59 @@ Record dir_names :=
 Context (P: dir.t → iProp Σ).
 Implicit Types (σ: dir.t) (γ: dir_names).
 
+(** Per-inode statements and lemmas about them. *)
+Local Definition inode_blocks γblocks (idx: nat) (blocks: list Block): iProp Σ :=
+  own γblocks (◯ {[ idx := Excl blocks ]}: blocksR).
+Local Definition inode_allblocks γblocks (allblocks: gmap nat (list Block)): iProp Σ :=
+  own γblocks (● (Excl <$> allblocks): blocksR).
+Local Definition inode_used γused (idx: nat) (used: gset u64): iProp Σ :=
+  own γused (◯ {[ idx := Excl used ]}: allocsR).
+Local Definition inode_allused γused (allused: gmap nat (gset u64)): iProp Σ :=
+  own γused (● (Excl <$> allused): allocsR).
+
+Lemma inode_blocks_lookup γblocks (idx: nat) (blocks: list Block) (allblocks: gmap nat (list Block)):
+  inode_blocks γblocks idx blocks -∗
+  inode_allblocks γblocks allblocks -∗
+  ⌜allblocks !! idx = Some blocks⌝.
+Proof.
+  iIntros "Hblocks Hallblocks".
+  iDestruct (own_valid_2 with "Hallblocks Hblocks") as
+      %[Hincl _]%auth_both_valid.
+  iPureIntro.
+  move: Hincl. rewrite singleton_included_l=> -[oblocks []].
+  rewrite lookup_fmap fmap_Some_equiv=> -[blocks' [-> ->]].
+  rewrite Excl_included leibniz_equiv_iff => -> //.
+Qed.
+
+Lemma inode_used_lookup γused (idx: nat) (used: gset u64) (allused: gmap nat (gset u64)):
+  inode_used γused idx used -∗
+  inode_allused γused allused -∗
+  ⌜allused !! idx = Some used⌝.
+Proof.
+  iIntros "Hused Hallused".
+  iDestruct (own_valid_2 with "Hallused Hused") as
+      %[Hincl _]%auth_both_valid.
+  iPureIntro.
+  move: Hincl. rewrite singleton_included_l=> -[oused []].
+  rewrite lookup_fmap fmap_Some_equiv=> -[used' [-> ->]].
+  rewrite Excl_included leibniz_equiv_iff => -> //.
+Qed.
+
 (** Protocol invariant for inode library *)
-Local Definition Pinode γblocks γused (s: inode.t) (idx: nat): iProp Σ :=
-  "Hownblocks" ∷ own γblocks (◯ {[ idx := Excl s.(inode.blocks) ]}: blocksR) ∗
-  "Hused1" ∷ own γused (◯ {[ idx := Excl s.(inode.addrs) ]} : allocsR).
+Local Definition Pinode γblocks γused (idx: nat) (s: inode.t): iProp Σ :=
+  "Hownblocks" ∷ inode_blocks γblocks idx s.(inode.blocks) ∗
+  "Hused1" ∷ inode_used γused idx s.(inode.addrs).
 
 (** Protocol invariant for alloc library *)
 Local Definition Palloc γused (s: alloc.t): iProp Σ :=
   ∃ allocs: gmap nat (gset u64), (* per-inode used blocks *)
     "%Hused_global" ∷ ⌜alloc.used s = ⋃ (snd <$> map_to_list allocs)⌝ ∗
-    "Hused2" ∷ own γused (● (Excl <$> allocs) : allocsR).
+    "Hused2" ∷ inode_allused γused allocs.
 
 (** Our own invariant (added to this is [P dir]) *)
 Definition dir_inv γblocks (dir: dir.t): iProp Σ :=
   "%Hdom" ∷ ⌜ dom (gset nat) dir.(dir.inodes) = list_to_set (seq 0 5) ⌝ ∗
-  "Hγblocks" ∷ own γblocks (● (Excl <$> dir.(dir.inodes)) : blocksR).
+  "Hγblocks" ∷ inode_allblocks γblocks dir.(dir.inodes).
 
 (** In-memory state of the directory (persistent) *)
 Definition is_dir (l: loc) γ: iProp Σ :=
